dev/lf/delayed-types/Canonical_forms2.v
@@ -98,7 +98,7 @@ Proof.
   pose proof (general_to_tight_typing Hg Hty) as Hty'.
   pose proof (tight_to_precise_trm_dec Hg Hty') as [T' [Hx Hs]].
   pose proof (corresponding_types Hwf Hg Bi)
-    as [[L [U [W [S1 [W1 [t [Hb [Ht [Heq [Hs1 Hs2]]]]]]]]]] | [[U [ds [Hb [Ht Heq]]]] | [U [l [Hb [Ht Heq]]]]]].
+    as [[L [U [W [S1 [W1 [t [Hb [Ht [Heq [Hs1 Hs2]]]]]]]]]] | [[U [ds [Hb [Ht Heq]]]] | [[U [l [Hb [Ht Heq]]]] | [U [Hb [Ht Heq]]]]]].
   + assert (H: exists T, record_type T /\ V = (typ_bnd T)).
     { pose proof (inert_binds Hg Bi) as Hgt.
       induction Hgt.
@@ -118,6 +118,16 @@ Proof.
     split; auto.
     apply tight_to_general in Hs; auto.
     apply ty_sub with (T:=T'); auto.
+  + assert (H: exists T, record_type T /\ V = (typ_bnd T)).
+    { pose proof (inert_binds Hg Bi) as Hgt.
+      induction Hgt.
+      - pose proof (precise_flow_lemma Bi Hx) as H.
+        apply (precise_flow_all_inv) in H.
+        inversion H.
+      - exists T0. auto.
+    }
+    destruct H as [T0 [Hrt Hsubst]]; subst V; rename T0 into V.
+    inversion Hsubst.
   + assert (H: exists T, record_type T /\ V = (typ_bnd T)).
     { pose proof (inert_binds Hg Bi) as Hgt.
       induction Hgt.
