dev/lf/delayed-types/Substitution.v
@@ -24,6 +24,7 @@ Fixpoint subst_typ (z: var) (u: var) (T: typ) { struct T } : typ :=
   | typ_bnd T      => typ_bnd (subst_typ z u T)
   | typ_all T U    => typ_all (subst_typ z u T) (subst_typ z u U)
   | typ_ref T      => typ_ref (subst_typ z u T)
+  | typ_nref T     => typ_nref (subst_typ z u T)
   end
 with subst_dec (z: var) (u: var) (D: dec) { struct D } : dec :=
   match D with
@@ -38,7 +39,7 @@ Fixpoint subst_trm (z: var) (u: var) (t: trm) : trm :=
   | trm_sel x1 L     => trm_sel (subst_avar z u x1) L
   | trm_app x1 x2    => trm_app (subst_avar z u x1) (subst_avar z u x2)
   | trm_let t1 t2    => trm_let (subst_trm z u t1) (subst_trm z u t2)
-  | trm_ref x t      => trm_ref (subst_avar z u x) (subst_typ z u t)
+  | trm_ref T        => trm_ref (subst_typ z u T)
   | trm_deref x      => trm_deref (subst_avar z u x)
   | trm_asg x y      => trm_asg (subst_avar z u x) (subst_avar z u y)
   end
@@ -47,6 +48,7 @@ with subst_val (z: var) (u: var) (v: val) : val :=
   | val_new T ds     => val_new (subst_typ z u T) (subst_defs z u ds)
   | val_lambda T t   => val_lambda (subst_typ z u T) (subst_trm z u t)
   | val_loc l        => val_loc l
+  | val_null         => val_null
   end
 with subst_def (z: var) (u: var) (d: def) : def :=
   match d with
@@ -362,15 +364,16 @@ Proof.
     simpl. eapply ty_and1; eauto.
   - (* ty_and2 *)
     simpl. eapply ty_and2; eauto.
-  - (* ty_ref_intro *)
-    simpl. constructor.
-    assert (trm_var (avar_f (If x = x0 then y else x)) = subst_trm x0 y (trm_var (avar_f x))) as A by (simpl; reflexivity).
-    rewrite A.
-    apply H; auto.
+  - (* ty_ref_intro *) 
+    simpl. apply ty_ref_intro with (x:=(If x = x0 then y else x)). apply H; auto.
   - (* ty_ref_elim *)
     apply ty_ref_elim; eauto.
-  - (* ty_asgn *)
-    apply ty_asgn; eauto.
+  - (* ty_asgn_ref *)
+    apply ty_asgn_ref; eauto.
+  - (* ty_asgn_nref *)
+    apply ty_asgn_nref; eauto.
+  - (* ty_null *)
+    constructor.
   - (* ty_def_typ *)
     simpl. apply ty_def_typ; auto.
   - (* ty_def_trm *)
@@ -424,7 +427,10 @@ Proof.
     rewrite concat_assoc. apply ok_push. assumption. auto.
     rewrite <- B. rewrite concat_assoc. apply weaken_ty_trm_ctx. assumption.
     apply ok_push. apply ok_concat_map. auto. unfold subst_env. auto.
-  - (* subtyp_ref *) apply subtyp_ref; auto.
+  - (* subtyp_ref *) 
+    apply subtyp_ref; auto.
+  - (* subtyp_nref *)
+    constructor.
 Qed.
 
 Lemma subst_ty_trm: forall y V G S x t T,
