dev/lf/delayed-types/Tight_possible_types.v
@@ -68,6 +68,10 @@ Inductive tight_pt : ctx -> sigma -> var -> typ -> Prop :=
   subtyp ty_general sub_tight G S T U ->
   subtyp ty_general sub_tight G S U T ->  
   tight_pt G S x (typ_ref U)
+  (* Nullable ref *)
+| t_pt_nref : forall G S x T,
+  tight_pt G S x (typ_ref T) ->
+  tight_pt G S x (typ_nref T)
   (* Top *)
 | t_pt_top : forall G S x T,
   tight_pt G S x T ->
